Refactoring some code

AVLtree.dfy
@@ -1,26 +1,28 @@
 datatype AVLnode = Leaf  |  Node (leftNode: AVLnode, height: nat, number: int, rightNode: AVLnode)
 
 /* Ensure the AVL tree is a binary search tree */
-predicate BST(left:AVLnode, x:int, right:AVLnode) 
+predicate BST(leftTree:AVLnode, number:int, rightTree:AVLnode)
 {
-    (forall i :: i in get_numbers(left) ==> i < x) && 
-    (forall j :: j in get_numbers(right) ==> x < j)
+    var leftNumbers := get_numbers(leftTree);
+    var rightNumbers := get_numbers(rightTree);
+    (forall i: int :: i in leftNumbers ==> i < number) && 
+    (forall j: int :: j in rightNumbers ==> number < j)
 }
 
 /* Function that returns the numbers in an AVL tree in order */
-function get_numbers(t:AVLnode): set<int>
-decreases t
+function get_numbers(currNode:AVLnode): set<int>
+decreases currNode
 {
-    if t == Leaf then
+    if currNode == Leaf then
         {}
     else
-        get_numbers(t.leftNode) + {t.number} + get_numbers(t.rightNode)
+        get_numbers(currNode.leftNode) + get_numbers(currNode.rightNode) + {currNode.number}
 }
 
 function get_node_height(node:AVLnode): nat
 {
     if(node == Leaf) then
-            0
+        0
     else
         node.height
 }
